defined type descriptions and elements of type descriptions

theories/Ref/SpecM.v
@@ -1,17 +1,9 @@
-From ITree Require Import
-     Basics.Basics
-     Basics.Tacs
-     Basics.HeterogeneousRelations
-     Basics.Monad
- .
+
 From EnTree Require Import
      Basics.HeterogeneousRelations
      Basics.QuantType
-     Basics.PolyList
      Core.EnTreeDefinition
      Core.SubEvent
-     Eq.Eqit
-     Ref.Padded
      Ref.EnTreeSpecDefinition
      Ref.FixTree
 .
@@ -19,19 +11,10 @@ From Coq Require Import
   Arith.Arith
   Strings.String
   Lists.List
-  Logic.Eqdep_dec
-  Logic.EqdepFacts
-  Eqdep EqdepFacts
-  Morphisms
+  Logic.FunctionalExtensionality
 .
 
-From Paco Require Import paco.
-
-Local Open Scope entree_scope.
-Local Open Scope list_scope.
-
 Import Monads.
-Import ProperNotations.
 
 
 (**
@@ -69,6 +52,278 @@ Global Instance ReSumRet_SpecE_Error (E : EvType) : ReSumRet ErrorE (SpecE E) :=
 
 
 (**
+ ** Type Descriptions
+ **)
+
+Variant ArithKind : Type@{entree_u} :=
+| Kind_Nat
+| Kind_BV (w:nat)
+.
+
+Variant KindDesc : Type@{entree_u} :=
+| Kind_Arith (K:ArithKind)
+| Kind_Tp
+.
+
+Variant ArithUnOp := | Op1_Neg | Op1_Succ.
+Variant ArithBinOp := | Op2_Plus | Op2_Times.
+
+Inductive CastOp : ArithKind -> ArithKind -> Type@{entree_u} :=
+| Cast_BVToNat w : CastOp (Kind_BV w) Kind_Nat
+| Cast_NatToBV w : CastOp Kind_Nat (Kind_BV w)
+| Cast_BVResize w1 w2 : CastOp (Kind_BV w1) (Kind_BV w2).
+
+Inductive ArithConst : ArithKind -> Type@{entree_u} :=
+| Const_nat (n:nat) : ArithConst Kind_Nat
+| Const_bv (w:nat) (bits:VectorDef.t bool w) : ArithConst (Kind_BV w).
+
+Inductive ArithExpr (K:ArithKind) : Type@{entree_u} :=
+| Arith_Const (c:ArithConst K)
+| Arith_Var (ix:nat)
+| Arith_UnOp (op:ArithUnOp) (e:ArithExpr K)
+| Arith_BinOp (op:ArithBinOp) (e1 e2:ArithExpr K)
+| Arith_Cast K' (op:CastOp K' K) (e:ArithExpr K')
+.
+
+(* The natural number 0 as an ArithExpr *)
+Definition ArithZ : ArithExpr Kind_Nat := Arith_Const _ (Const_nat 0).
+
+(* The successor function on ArithExprs *)
+Definition ArithS (e: ArithExpr Kind_Nat) : ArithExpr Kind_Nat :=
+  Arith_UnOp _ Op1_Succ e.
+
+(* Descriptions of types *)
+Inductive TpDesc : Type@{entree_u} :=
+(* Monadic function types *)
+| Tp_M (R : TpDesc)
+| Tp_Pi (A : KindDesc) (B : TpDesc)
+| Tp_Arr (A : TpDesc) (B : TpDesc)
+
+(* First-order types *)
+| Tp_Kind (K : KindDesc)
+| Tp_Pair (A : TpDesc) (B : TpDesc)
+| Tp_Sum (A : TpDesc) (B : TpDesc)
+| Tp_Sigma (K : KindDesc) (B : TpDesc)
+| Tp_Vec (A : TpDesc) (n:ArithExpr Kind_Nat)
+
+(* Inductive types and type variables *)
+| Tp_Ind (A : TpDesc)
+| Tp_Var (n : nat)
+| Tp_Void
+.
+
+(**
+ ** Deciding equality of type descriptions
+ **)
+
+Lemma dec_eq_KindDesc (K1 K2:KindDesc) : {K1=K2} + {~K1=K2}.
+Proof. repeat decide equality. Qed.
+
+Lemma dec_eq_ArithConst_dep K1 (e1:ArithConst K1) K2 (e2:ArithConst K2) :
+  { existT ArithConst K1 e1 = existT ArithConst K2 e2 } +
+    { ~ existT ArithConst K1 e1 = existT ArithConst K2 e2 }.
+Proof.
+Admitted.
+
+Lemma dec_eq_ArithConst K (e1 e2:ArithConst K) : {e1=e2} + {~e1=e2}.
+Admitted.
+
+Lemma dec_eq_ArithExpr K (e1 e2 : ArithExpr K) : {e1=e2} + {~e1=e2}.
+Proof.
+  revert e2; induction e1; intro e2; destruct e2; try (right; intro H; discriminate H).
+  - destruct (dec_eq_ArithConst K c c0).
+    + rewrite e; left; reflexivity.
+    + right; intro H; inversion H; apply n; assumption.
+  - destruct (Nat.eq_dec ix ix0).
+    + rewrite e; left; reflexivity.
+    + right; intro H; inversion H; apply n; assumption.
+Admitted.
+
+Definition dec_eq_TpDesc (T U:TpDesc) : { T = U } + {~ T = U}.
+Proof.
+  repeat decide equality. apply dec_eq_ArithExpr.
+Qed.
+
+
+(**
+ ** Elements of kind descriptions
+ **)
+
+Definition arithKindElem K :=
+  match K with
+  | Kind_Nat => nat
+  | Kind_BV w => VectorDef.t bool w
+  end.
+
+(* An element of a kind *)
+Definition kindElem K : Type@{entree_u} :=
+  match K with
+  | Kind_Tp => TpDesc
+  | Kind_Arith K' => arithKindElem K'
+  end.
+
+Definition defaultKindElem K : kindElem K :=
+  match K return kindElem K with
+  | Kind_Arith Kind_Nat => 0
+  | Kind_Arith (Kind_BV w) => VectorDef.const false w
+  | Kind_Tp => Tp_Void
+  end.
+
+
+(**
+ ** Substitution for type descriptions
+ **)
+
+(* An element of an environment is a value, i.e., an element of some kind *)
+Definition TpEnvElem : Type@{entree_u} := { K & kindElem K }.
+
+(* An environment is a substitution from variables to values *)
+Definition TpEnv := list TpEnvElem.
+
+(* Add a value to a type environment *)
+Definition envConsElem {K} (elem:kindElem K) (env:TpEnv) : TpEnv :=
+  cons (existT kindElem K elem) env.
+
+(* Eliminate a TpEnvElem at a particular kind, returning the default element of
+that kind if the kind of the head does not match *)
+Definition elimTpEnvElem K (elem:TpEnvElem) : kindElem K :=
+  match dec_eq_KindDesc (projT1 elem) K with
+  | left e => eq_rect (projT1 elem) kindElem (projT2 elem) K e
+  | right _ => defaultKindElem K
+  end.
+
+(* Get the head value of a TpEnv at a particular kind, returning the default
+element of that kind if the kind of the head does not match or env is empty *)
+Definition headTpEnv K (env:TpEnv) : kindElem K :=
+  match env with
+  | nil => defaultKindElem K
+  | elem :: _ => elimTpEnvElem K elem
+  end.
+
+(* Turn an element of an arith kind into an expression *)
+Definition arithKindElemExpr {K} : arithKindElem K -> ArithExpr K :=
+  match K return arithKindElem K -> ArithExpr K with
+  | Kind_Nat => fun n => Arith_Const _ (Const_nat n)
+  | Kind_BV w => fun bv => Arith_Const _ (Const_bv w bv)
+  end.
+
+
+(* Evaluate a variable of a particular kind relative to an environment at a
+given lifting level n, meaning that the environment is a substitution for the
+variables starting at n *)
+Fixpoint substVar n env K var {struct var} : kindElem K + nat :=
+  match var with
+  | 0 => match n with
+         | 0 => inl (headTpEnv K env)
+         | S _ => inr 0
+         end
+  | S var' =>
+      match n with
+      | 0 => substVar 0 (tail env) K var'
+      | S n' =>
+          match substVar n' env K var' with
+          | inl ret =>
+              (* NOTE: if we were doing lifting, this is where we would do it *)
+              inl ret
+          | inr v_ret => inr (S v_ret)
+          end
+      end
+  end.
+
+(* Evaluate a variable to a value, using the default value for free variables *)
+Definition evalVar n env K var : kindElem K :=
+  match substVar n env K var with
+  | inl v => v
+  | inr _ => defaultKindElem K
+  end.
+
+(* Substitute an environment at lifting level n into arithmetic expression e *)
+Fixpoint substArithExpr n env {K'} (e:ArithExpr K') : ArithExpr K' :=
+  match e with
+  | Arith_Const _ c => Arith_Const _ c
+  | Arith_Var _ ix =>
+      match substVar n env (Kind_Arith K') ix with
+      | inl e' => arithKindElemExpr e'
+      | inr ix' => Arith_Var _ ix'
+      end
+  | Arith_UnOp _ op e' => Arith_UnOp _ op (substArithExpr n env e')
+  | Arith_BinOp _ op e1 e2 =>
+      Arith_BinOp _ op (substArithExpr n env e1) (substArithExpr n env e2)
+  | Arith_Cast _ K' op e' => Arith_Cast _ _ op (substArithExpr n env e')
+  end.
+
+(* Substitute an environment at lifting level n into type description T *)
+Fixpoint tpSubst n env (T:TpDesc) : TpDesc :=
+  match T with
+  | Tp_M R => Tp_M (tpSubst n env R)
+  | Tp_Pi A B => Tp_Pi A (tpSubst (S n) env B)
+  | Tp_Arr A B => Tp_Arr (tpSubst n env A) (tpSubst n env B)
+  | Tp_Kind K => Tp_Kind K
+  | Tp_Pair A B => Tp_Pair (tpSubst n env A) (tpSubst n env B)
+  | Tp_Sum A B => Tp_Sum (tpSubst n env A) (tpSubst n env B)
+  | Tp_Sigma A B => Tp_Sigma A (tpSubst (S n) env B)
+  | Tp_Vec A e => Tp_Vec (tpSubst n env A) (substArithExpr n env e)
+  | Tp_Ind A => Tp_Ind (tpSubst (S n) env A)
+  | Tp_Var var => match substVar n env Kind_Tp var with
+                  | inl U => U
+                  | inr var' => Tp_Var var'
+                  end
+  | Tp_Void => Tp_Void
+  end.
+
+
+(**
+ ** Elements of type descriptions
+ **)
+
+Fixpoint evalArithExpr (env:TpEnv) {K} (e:ArithExpr K) : arithKindElem K.
+Admitted.
+
+(* Inductively defined elements of a type description *)
+Inductive indElem : TpEnv -> TpDesc -> Type@{entree_u} :=
+| Elem_M {env R} (f:FunIx (Tp_M R)) : indElem env (Tp_M R)
+| Elem_Pi {env A B} (f:FunIx (Tp_Pi A B)) : indElem env (Tp_Pi A B)
+| Elem_Arr {env A B} (f:FunIx (Tp_Arr A B)) : indElem env (Tp_Arr A B)
+| Elem_Kind {env K} (elem:kindElem K) : indElem env (Tp_Kind K)
+| Elem_Pair {env A B} (elem1: indElem env A) (elem2: indElem env B)
+  : indElem env (Tp_Pair A B)
+| Elem_SumL {env A B} (elem: indElem env A) : indElem env (Tp_Sum A B)
+| Elem_SumR {env A B} (elem: indElem env B) : indElem env (Tp_Sum A B)
+| Elem_Sigma {env K B}
+    (elem1: kindElem K) (elem2: indElem (envConsElem elem1 env) B)
+  : indElem env (Tp_Sigma K B)
+| Elem_VecNil {env A} : indElem env (Tp_Vec A ArithZ)
+| Elem_VecCons {env A e} (elem1: indElem env A) (elem2: indElem env (Tp_Vec A e))
+  : indElem env (Tp_Vec A (ArithS e))
+| Elem_VecCast {env A e1 e2} (e: evalArithExpr env e1 = evalArithExpr env e2)
+    (elem: indElem env (Tp_Vec A e1)) : indElem env (Tp_Vec A e2)
+| Elem_Ind {env A} (elem: indElem (@envConsElem Kind_Tp
+                                     (tpSubst 0 env (Tp_Ind A))
+                                     env) A)
+  : indElem env (Tp_Ind A)
+| Elem_Var {env} var (elem: indElem nil (evalVar 0 env Kind_Tp var)) :
+  indElem env (Tp_Var var)
+(* No case for Tp_Void *)
+.
+
+(* Elements of a type description *)
+Fixpoint tpElem env T : Type@{entree_u} :=
+  match T with
+  | Tp_M R => FunIx (Tp_M R)
+  | Tp_Pi K B => FunIx (Tp_Pi K B)
+  | Tp_Arr A B => FunIx (Tp_Arr A B)
+  | Tp_Kind K => kindElem K
+  | Tp_Pair A B => tpElem env A * tpElem env B
+  | Tp_Sum A B => tpElem env A + tpElem env B
+  | Tp_Sigma K B => { elem: kindElem K & tpElem (envConsElem elem env) B }
+  | Tp_Vec A e => VectorDef.t (tpElem env A) (evalArithExpr env e)
+  | Tp_Ind A => indElem env (Tp_Ind A)
+  | Tp_Var var => indElem nil (evalVar 0 env Kind_Tp var)
+  | Tp_Void => Empty_set
+  end.
+
+
+(**
  ** The SpecM monad
  **)
 
@@ -103,7 +358,7 @@ Definition ErrorS {A} (str : string) : SpecM A :=
     (fun (x:Empty_set) => match x with end).
 
 Definition errorEntree {R} (s : string) : entree (SpecEv E) R :=
-  Vis (Spec_vis (inl (mkErrorE s))) (fun v:void => match v with end).
+  Vis (Spec_vis (inl (mkErrorE s))) (fun v:Empty_set => match v with end).
 
 Definition interp_SpecM {R} (t:SpecM R) : entree (SpecEv E) R :=
   interp_fixtree (@errorEntree R "Unbound function call") nil t.
